trusted/SMT-prove.lisp
@@ -13,45 +13,51 @@
 (include-book "../verified/SMT-hint-interface")
 (include-book "../verified/SMT-config")
 
-;; (defsection SMT-prove
-;;   :parents (Smtlink)
-;;   :short "SMT-prove is the main functions for transliteration into SMT languages and calling the external SMT solver."
+(defsection SMT-prove
+  :parents (Smtlink)
+  :short "SMT-prove is the main functions for transliteration into SMT languages and calling the external SMT solver."
 
-;; ;; (defun mk-fname (directory fname-LISP suffix)
-;; ;;   (let ((dir (if (equal directory "") "/tmp/py_file" directory)))
-;; ;;     (cond ((equal fname-LISP "")
-;; ;;            (let ((cmd (concatenate 'string "mkdir -p " dir " && "
-;; ;;                                    "mktemp " dir "/smtlink" suffix ".XXXXX")))
-;; ;;              (mv-let (exit-status lines)
-;; ;;                (time$ (tshell-call cmd
-;; ;;                                    :print t
-;; ;;                                    :save t)
-;; ;;                       :msg "; mktemp: `~s0`: ~st sec, ~sa bytes~%"
-;; ;;                       :args (list cmd))
-;; ;;                (if (equal exit-status 0)
-;; ;;                    (car lines)
-;; ;;                  (er hard? 'top-level "Error: Generate file error.")))))
-;; ;;           ((stringp fname-LISP)
-;; ;;            (concatenate 'string dir "/" (string (lisp-to-python-names fname-LISP)) suffix))
-;; ;;           (t (er hard? 'top-level "Error: fname should either be a string or \"\"")))))
+;; (defun mk-fname (directory fname-LISP suffix)
+;;   (let ((dir (if (equal directory "") "/tmp/py_file" directory)))
+;;     (cond ((equal fname-LISP "")
+;;            (let ((cmd (concatenate 'string "mkdir -p " dir " && "
+;;                                    "mktemp " dir "/smtlink" suffix ".XXXXX")))
+;;              (mv-let (exit-status lines)
+;;                (time$ (tshell-call cmd
+;;                                    :print t
+;;                                    :save t)
+;;                       :msg "; mktemp: `~s0`: ~st sec, ~sa bytes~%"
+;;                       :args (list cmd))
+;;                (if (equal exit-status 0)
+;;                    (car lines)
+;;                  (er hard? 'top-level "Error: Generate file error.")))))
+;;           ((stringp fname-LISP)
+;;            (concatenate 'string dir "/" (string (lisp-to-python-names fname-LISP)) suffix))
+;;           (t (er hard? 'top-level "Error: fname should either be a string or \"\"")))))
 
 ;; ;; (defun write-SMT-file (py-term smt-file)
 ;; ;;   (declare (ignore py-term smt-file))
 ;; ;;   )
 
-;;   (defun SMT-prove (term smtlink-hint)
-;;     (b* ((fname (smtlink-hint->python-file (smt-hint)))
-;;          (uninterpreted (smtlink-hint->uninterpreted (smt-hint)))
-;;          (directory (smtlink-config->SMT-files-dir (smt-cnf)))
-;;          (file-format (smtlink-config->file-format (smt-cnf)))
-;;          (smt-file (mk-fname directory fname file-format))
+  (define SMT-prove ((term pseudo-term-listp) (smtlink-hint smtlink-hint-p))
+    :ignore-ok t
+    :returns (proved? booleanp)
+    (b* ((term (mbe :logic (pseudo-term-list-fix term) :exec term))
+         (smtlink-hint (mbe :logic (smtlink-hint-fix smtlink-hint) :exec smtlink-hint))
+         ((smtlink-hint h) smtlink-hint)
+         ((smtlink-config c) h.smt-cnf)
+         (fname h.python-file)
+         (dir c.SMT-files-dir)
+         (format c.file-format)
 
-;;          (translated-py-term (SMT-transliteration term))
+         ;; (uninterpreted (smtlink-hint->uninterpreted (smt-hint)))
+         ;; (smt-file (mk-fname directory fname file-format))
 
-;;          (state (write-SMT-file translated-py-term smt-file))
+         ;; (translated-py-term (SMT-transliteration term))
 
-;;          (result (run-SMT-solver smt-file))))
-;;     result)
-;; )
-(define SMT-prove (term smtlink-hint)
-  (or term smtlink-hint t))
+         ;; (state (write-SMT-file translated-py-term smt-file))
+
+         ;; (result (run-SMT-solver smt-file))
+         (result t))
+      result))
+)
